examples/low-level/crypto/Crypto.WIP.fst
@@ -99,13 +99,96 @@ let lemma_frame_find_mac (#i:PRF.id) (#l:nat) (st:PRF.state i)
 		      let x0 = {x with ctr=0ul} in
 		      find_mac tab0 x0 == find_mac tab1 x0)))
     = admit()		      
+
+open FStar.Heap
+let heap_modifies_fresh_empty_0  (h0:heap) (h1:heap) (h2:heap) (x:FStar.Heap.ref nat)
+  : Lemma (requires (Heap.modifies TSet.empty h0 h1 /\
+		     Heap.modifies !{x} h1 h2 /\
+		     not(h0 `Heap.contains` x)))
+          (ensures (Heap.modifies TSet.empty h0 h2))
+  = ()	  
+
+let modifies_fresh_empty_0  (h0:mem) (h1:mem) (h2:mem) (r:rid) (x:HS.reference nat)
+  : Lemma (requires (HS (h0.h) `Map.contains` r /\
+		     HS.modifies_ref r TSet.empty h0 h1 /\
+  		     HS.modifies_ref r (TSet.singleton (HS.as_aref x)) h1 h2 /\
+		     HS.frameOf x == r /\
+		     ~(h0 `HS.contains` x)))
+          (ensures (HS.modifies_ref r TSet.empty h0 h2))
+  = ()	  
+  
+let modifies_fresh_empty (i:id) (n: Cipher.iv (alg i)) (r:rid) (m:MAC.state (i,n)) 
+			 (h0:mem) (h1:mem) (h2:mem) 
+  : Lemma (requires (HS (h0.h) `Map.contains` r /\
+		     HS.modifies_ref r TSet.empty h0 h1 /\
+		    (mac_log ==> 
+		        (let ref = MAC (as_hsref (ilog m.log)) in
+			 HS.frameOf ref == r /\
+			 HS.modifies_ref r (TSet.singleton (MAC (HS.as_aref ref))) h1 h2)) /\
+		    (safeId i ==> ~ (m_contains (MAC (ilog m.log)) h0))))
+          (ensures (safeId i ==> HS.modifies_ref r TSet.empty h0 h2))
+  = assert (safeId i ==> prf i /\ mac_log);
+    ()
+  
+#reset-options "--z3timeout 400 --initial_fuel 0 --max_fuel 0 --initial_ifuel 0 --max_ifuel 0 --log_queries"
+
+val extend_refines_aux: (i:id) -> (st:state i Writer) -> (nonce:Cipher.iv (alg i)) ->
+		       (aadlen: UInt32.t {aadlen <=^ aadmax}) ->
+		       (aad: lbuffer (v aadlen)) ->
+                       (len:nat{len<>0}) -> (plain:plainBuffer i len) -> (cipher:lbuffer (len + v (Spec.taglen i))) ->
+		       (h0:mem) ->
+                       (h1:mem{Buffer.live h1 aad /\ Plain.live h1 plain /\ Buffer.live h1 cipher}) ->
+    Lemma (requires ( safeId i ==> (
+		      let mac_rgn = st.prf.mac_rgn in
+      		      let entries_0 = HS.sel h0 st.log in 
+		      let blocks_0 = HS.sel h0 (PRF.itable i st.prf) in
+		      let table_1 = HS.sel h1 (PRF.itable i st.prf) in
+		      Seq.length table_1 > Seq.length blocks_0 /\ (
+		      let blocks_1 = Seq.slice table_1 (Seq.length blocks_0) (Seq.length table_1) in
+
+     		      let p = Plain.sel_plain h1 (u len) plain in
+		      let c_tagged = Buffer.as_seq h1 cipher in
+	              let c, tag = SeqProperties.split c_tagged len in
+		      let ad = Buffer.as_seq h1 aad in
+  		      let entry = Entry nonce ad len p c_tagged in
+		      pre_refines_one_entry i st nonce len plain cipher h0 h1 /\
+		      inv h0 st /\
+		      refines_one_entry #_ #i h1 entry blocks_1 /\
+      		      HS.modifies_ref mac_rgn TSet.empty h0 h1 /\
+		      HS.live_region h1 mac_rgn))))
+		      
+          (ensures ( safeId i ==> (
+		      let mac_rgn = st.prf.mac_rgn in
+      		      let entries_0 = HS.sel h0 st.log in 
+		      let table_1 = HS.sel h1 (PRF.itable i st.prf) in
+     		      let p = Plain.sel_plain h1 (u len) plain in
+		      let c_tagged = Buffer.as_seq h1 cipher in
+	              let c, tag = SeqProperties.split c_tagged len in
+		      let ad = Buffer.as_seq h1 aad in
+  		      let entry = Entry nonce ad len p c_tagged in
+		      refines h1 i mac_rgn (SeqProperties.snoc entries_0 entry) table_1)))
+let extend_refines_aux i st nonce aadlen aad len plain cipher h0 h1 = 
+  if safeId i then
+     let mac_rgn = st.prf.mac_rgn in
+     let entries_0 = HS.sel h0 st.log in 
+     let blocks_0 = HS.sel h0 (PRF.itable i st.prf) in
+     let table_1 = HS.sel h1 (PRF.itable i st.prf) in
+     let blocks_1 = Seq.slice table_1 (Seq.length blocks_0) (Seq.length table_1) in
+     let p = Plain.sel_plain h1 (u len) plain in
+     let c_tagged = Buffer.as_seq h1 cipher in
+     let c, tag = SeqProperties.split c_tagged len in
+     let ad = Buffer.as_seq h1 aad in
+     let entry = Entry nonce ad len p c_tagged in
+     assume (pre_refines_one_entry i st nonce len plain cipher h0 h1);
+     extend_refines h0 i mac_rgn entries_0 blocks_0 entry blocks_1 h1
  
-#reset-options "--z3timeout 400 --initial_fuel 0 --max_fuel 0 --initial_ifuel 0 --max_ifuel 0"
 let encrypt i st n aadlen aad plainlen plain cipher_tagged =
   (* push_frame(); *)
   (* assume (safeId i); *)
   (* assume (prf i); *)
   let h0 = get() in
+  assume (HS (h0.h `Map.contains` st.prf.mac_rgn));
+  assume (HS (HH.disjoint h0.tip st.prf.mac_rgn));
   assume (HS (is_stack_region h0.tip)); //TODO: remove this once we move all functions to STL
   let x = PRF({iv = n; ctr = 0ul}) in // PRF index to the first block
   let ak = PRF.prf_mac i st.prf x in  // used for keying the one-time MAC  
@@ -114,9 +197,9 @@ let encrypt i st n aadlen aad plainlen plain cipher_tagged =
   let cipher = Buffer.sub cipher_tagged 0ul plainlen in
   let tag = Buffer.sub cipher_tagged plainlen (Spec.taglen i) in
   let y = PRF.incr i x in
-  //calling this lemma allows us to complete the proof without using any fuel; 
+  //calling this lemma allows us to complete the proof without using any fuel;
   //which makes things a a bit faster
-  counterblocks_emp i st.prf.mac_rgn y (v plainlen) 0 
+  counterblocks_emp i st.prf.mac_rgn y (v plainlen) 0
       (Plain.sel_plain h1 plainlen plain) (Buffer.as_seq h1 cipher);
   counter_enxor i st.prf y plainlen plainlen plain cipher h1;
   // Compute MAC over additional data and ciphertext
@@ -130,30 +213,22 @@ let encrypt i st n aadlen aad plainlen plain cipher_tagged =
   let h3 = get() in
   Buffer.lemma_reveal_modifies_0 h2 h3;
   assert (HS.modifies_ref st.prf.mac_rgn TSet.empty h0 h3);
-  (* assume (HH.disjoint (HS.frameOf acc) st.prf.mac_rgn); *)
   frame_pre_refines_0 i st n (v plainlen) plain cipher_tagged h0 h2 h3;
-  (* let _ = *)
-  (*   let c = Buffer.as_seq h3 cipher in *)
-  (*   let ad = Buffer.as_seq h3 aad in *)
-  (*   assert (l == field_encode i ad #plainlen c) in *)
   assert (Buffer.live h2 aad); //seem to need this hint
   assert (Buffer.live h3 aad); //seem to need this hint
   Buffer.lemma_reveal_modifies_0 h2 h3;
   MAC.mac ak l acc tag;
   let h4 = get () in
   FStar.Classical.move_requires (Buffer.lemma_reveal_modifies_1 tag h3) h4;
-  //really should get this from the mods clause ... need to investigate
-  (* assume (mac_log ==> HS.modifies_ref st.prf.mac_rgn (TSet.singleton (MAC (HS.as_aref (as_hsref (ilog ak.log))))) h3 h4); *)
+  modifies_fresh_empty i n st.prf.mac_rgn ak h0 h3 h4;
+  assert (safeId i ==> HS.modifies_ref st.prf.mac_rgn TSet.empty h0 h4);
   frame_pre_refines i st n (v plainlen) plain cipher_tagged h0 h3 h4;
-  (* assert (Buffer.as_seq h3 cipher == Buffer.as_seq h4 cipher); *)
-  (* assert (Buffer.as_seq h3 aad == Buffer.as_seq h4 aad); *)
-  (* assert (Buffer.live h4 aad); *)
-  (* assert (Buffer.live h4 cipher_tagged); *)
-  (* assert (Plain.live h4 plain); *)
   intro_mac_refines i st n aad plain cipher_tagged h4;
   pre_refines_to_refines i st n aadlen aad (v plainlen) plain cipher_tagged h0 h4;
-  (* assert (safeId i /\ prf i /\ mac_log ==> HS.modifies_ref st.prf.mac_rgn TSet.empty h0 h4); *)
+  extend_refines_aux i st n aadlen aad (v plainlen) plain cipher_tagged h0 h4;
   admit()
+
+
   
   (* let _ = *)
   (*   let tab = HS.sel h4 (itable i st.prf) in *)
