examples/low-level/crypto/Crypto.AEAD.Encoding.fst
@@ -344,7 +344,9 @@ val accumulate:
   (ensures (fun h0 (l,a) h1 -> 
     Buffer.modifies_0 h0 h1 /\ // modifies only fresh buffers on the current stack
     ~ (h0 `Buffer.contains` a) /\
-    Buffer.live h1 aad /\ Buffer.live h1 cipher /\
+    Buffer.live h1 aad /\ 
+    Buffer.live h1 cipher /\
+    Buffer.frameOf a = h1.tip /\
     MAC.acc_inv st l a h1 /\
     (mac_log ==> l == encode_both aadlen (Buffer.as_seq h1 aad) plainlen (Buffer.as_seq h1 cipher))))
   // StackInline required for stack-allocated accumulator
