ulib/FStar.HyperStack.fst
@@ -261,7 +261,6 @@ unfold let mods (rs:some_refs) h0 h1 =
     modifies (normalize_term (regions_of_some_refs rs)) h0 h1
   /\ (forall (r:rid). modifies_ref r (normalize_term (refs_in_region r rs)) h0 h1)
 
-
 ////////////////////////////////////////////////////////////////////////////////
 #set-options "--initial_fuel 0 --max_fuel 0"
 let f (a:Type0) (b:Type0) (x:reference a) (x':reference a) 
@@ -280,3 +279,30 @@ let f (a:Type0) (b:Type0) (x:reference a) (x':reference a)
 					 (Set.singleton z.id))) h0 h1);
   assert (sel h0 x' == sel h1 x');
   assert (modifies_ref x.id (TSet.singleton (as_aref x)) h0 h1)
+
+(* let f2 (a:Type0) (b:Type0) (x:reference a) (y:reference b) *)
+(* 			   (h0:mem) (h1:mem) =  *)
+(*   assume (HH.disjoint (frameOf x) (frameOf y)); *)
+(*   assume (mods [Ref x; Ref y] h0 h1); *)
+(*  //-------------------------------------------------------------------------------- *)
+(*   assert (modifies_ref x.id (TSet.singleton (as_aref x)) h0 h1) *)
+
+(* let rec modifies_some_refs (i:some_refs) (rs:some_refs) (h0:mem) (h1:mem) : GTot Type0 = *)
+(*   match i with *)
+(*   | [] -> True *)
+(*   | Ref x::tl -> *)
+(*     let r = x.id in *)
+(*     (modifies_ref r (normalize_term (refs_in_region r rs)) h0 h1 /\ *)
+(*      modifies_some_refs tl rs h0 h1) *)
+
+(* unfold let mods_2 (rs:some_refs) h0 h1 = *)
+(*     modifies (normalize_term (regions_of_some_refs rs)) h0 h1 *)
+(*   /\ modifies_some_refs rs rs h0 h1 *)
+
+(* #reset-options "--log_queries --initial_fuel 0 --max_fuel 0 --initial_ifuel 0 --max_ifuel 0" *)
+(* #set-options "--debug FStar.HyperStack --debug_level print_normalized_terms" *)
+(* let f3 (a:Type0) (b:Type0) (x:reference a) *)
+(* 			   (h0:mem) (h1:mem) =  *)
+(*   assume (mods_2 [Ref x] h0 h1); *)
+(*  //-------------------------------------------------------------------------------- *)
+(*   assert (modifies_ref x.id (TSet.singleton (as_aref x)) h0 h1) *)
